theories/zoo/iris/base_logic/lib/ghost_list.v
@@ -1,0 +1,183 @@
+From iris.base_logic Require Import
+  lib.ghost_map.
+
+From zoo Require Import
+  prelude.
+From zoo.iris.bi Require Import
+  big_op.
+From zoo.iris.base_logic Require Export
+  lib.base.
+From zoo.iris Require Import
+  diaframe.
+From zoo Require Import
+  options.
+
+Class GhostListG Σ V := {
+  #[local] ghost_list_G_map_G :: ghost_mapG Σ nat V ;
+}.
+
+Definition ghost_list_Σ V := #[
+  ghost_mapΣ nat V
+].
+#[global] Instance subG_ghost_list_Σ Σ V :
+  subG (ghost_list_Σ V) Σ →
+  GhostListG Σ V.
+Proof.
+  solve_inG.
+Qed.
+
+Section ghost_list_G.
+  Context `{ghost_list_G : !GhostListG Σ V}.
+
+  Definition ghost_list_auth γ vs :=
+    ghost_map_auth γ 1 (map_seq 0 vs).
+  Definition ghost_list_at γ :=
+    ghost_map_elem γ.
+
+  #[global] Instance ghost_list_auth_timeless γ vs :
+    Timeless (ghost_list_auth γ vs).
+  Proof.
+    apply _.
+  Qed.
+  #[global] Instance ghost_list_at_timeless γ i dq v :
+    Timeless (ghost_list_at γ i dq v).
+  Proof.
+    apply _.
+  Qed.
+  #[global] Instance ghost_list_at_persistent γ i v :
+    Persistent (ghost_list_at γ i DfracDiscarded v).
+  Proof.
+    apply _.
+  Qed.
+
+  #[global] Instance ghost_list_at_fractional γ i v :
+    Fractional (λ q, ghost_list_at γ i (DfracOwn q) v).
+  Proof.
+    apply _.
+  Qed.
+  #[global] Instance ghost_list_at_as_fractional γ i q v :
+    AsFractional (ghost_list_at γ i (DfracOwn q) v) (λ q, ghost_list_at γ i (DfracOwn q) v) q.
+  Proof.
+    apply _.
+  Qed.
+
+  Lemma ghost_list_alloc vs :
+    ⊢ |==>
+      ∃ γ,
+      ghost_list_auth γ vs ∗
+      [∗ list] i ↦ v ∈ vs,
+        ghost_list_at γ i (DfracOwn 1) v.
+  Proof.
+    iMod (ghost_map_alloc (map_seq 0 vs)) as "(%γ & $ & ?)".
+    rewrite big_sepM_map_seq_0 //.
+  Qed.
+
+  Lemma ghost_list_auth_exclusive γ vs1 vs2 :
+    ghost_list_auth γ vs1 -∗
+    ghost_list_auth γ vs2 -∗
+    False.
+  Proof.
+    iIntros "Hauth1 Hauth2".
+    iDestruct (ghost_map_auth_valid_2 with "Hauth1 Hauth2") as %(? & _). done.
+  Qed.
+
+  Lemma ghost_list_at_valid γ i dq v :
+    ghost_list_at γ i dq v ⊢
+    ⌜✓ dq⌝.
+  Proof.
+    iApply ghost_map_elem_valid.
+  Qed.
+  Lemma ghost_list_at_combine γ i dq1 v1 dq2 v2 :
+    ghost_list_at γ i dq1 v1 -∗
+    ghost_list_at γ i dq2 v2 -∗
+      ⌜v1 = v2⌝ ∗
+      ghost_list_at γ i (dq1 ⋅ dq2) v1.
+  Proof.
+    iIntros "Hat1 Hat2".
+    iDestruct (ghost_map_elem_combine with "Hat1 Hat2") as "($ & $)".
+  Qed.
+  Lemma ghost_list_at_valid_2 γ i dq1 v1 dq2 v2 :
+    ghost_list_at γ i dq1 v1 -∗
+    ghost_list_at γ i dq2 v2 -∗
+      ⌜✓ (dq1 ⋅ dq2)⌝ ∗
+      ⌜v1 = v2⌝.
+  Proof.
+    iIntros "Hat1 Hat2".
+    iDestruct (ghost_list_at_combine with "Hat1 Hat2") as "(-> & Hat)".
+    iDestruct (ghost_list_at_valid with "Hat") as "$".
+    iSteps.
+  Qed.
+  Lemma ghost_list_at_agree γ i dq1 v1 dq2 v2 :
+    ghost_list_at γ i dq1 v1 -∗
+    ghost_list_at γ i dq2 v2 -∗
+    ⌜v1 = v2⌝.
+  Proof.
+    iIntros "Hat1 Hat2".
+    iDestruct (ghost_list_at_valid_2 with "Hat1 Hat2") as "(_ & $)".
+  Qed.
+  Lemma ghost_list_at_dfrac_ne γ1 i1 dq1 v1 γ2 i2 dq2 v2 :
+    ¬ ✓ (dq1 ⋅ dq2) →
+    ghost_list_at γ1 i1 dq1 v1 -∗
+    ghost_list_at γ2 i2 dq2 v2 -∗
+    ⌜γ1 ≠ γ2 ∨ i1 ≠ i2⌝.
+  Proof.
+    rewrite -not_and_r. iIntros "% Hat1 Hat2 (-> & ->)".
+    iDestruct (ghost_list_at_valid_2 with "Hat1 Hat2") as "(% & _)". done.
+  Qed.
+  Lemma ghost_list_at_ne γ1 i1 v1 γ2 i2 dq2 v2 :
+    ghost_list_at γ1 i1 (DfracOwn 1) v1 -∗
+    ghost_list_at γ2 i2 dq2 v2 -∗
+    ⌜γ1 ≠ γ2 ∨ i1 ≠ i2⌝.
+  Proof.
+    iApply ghost_list_at_dfrac_ne; [done.. | intros []%(exclusive_l _)].
+  Qed.
+  Lemma ghost_list_at_exclusive γ i v1 dq2 v2 :
+    ghost_list_at γ i (DfracOwn 1) v1 -∗
+    ghost_list_at γ i dq2 v2 -∗
+    False.
+  Proof.
+    iIntros "Hat1 Hat2".
+    iDestruct (ghost_list_at_ne with "Hat1 Hat2") as %?. naive_solver.
+  Qed.
+  Lemma ghost_list_at_persist γ i dq v :
+    ghost_list_at γ i dq v ⊢ |==>
+    ghost_list_at γ i DfracDiscarded v.
+  Proof.
+    iApply ghost_map_elem_persist.
+  Qed.
+
+  Lemma ghost_list_lookup γ vs i dq v :
+    ghost_list_auth γ vs -∗
+    ghost_list_at γ i dq v -∗
+    ⌜vs !! i = Some v⌝.
+  Proof.
+    iIntros "Hauth Hat".
+    iDestruct (ghost_map_lookup with "Hauth Hat") as %?%(lookup_map_seq_Some_inv 0).
+    iSteps.
+  Qed.
+
+  Lemma ghost_list_update_push {γ vs} v :
+    ghost_list_auth γ vs ⊢ |==>
+      ghost_list_auth γ (vs ++ [v]) ∗
+      ghost_list_at γ (length vs) (DfracOwn 1) v.
+  Proof.
+    iIntros "Hauth".
+    iMod (ghost_map_insert (length vs) with "Hauth") as "(Hauth & $)".
+    { apply (map_seq_snoc_disjoint 0). }
+    rewrite -(map_seq_snoc 0) //.
+  Qed.
+  Lemma ghost_list_update_at {γ vs i w} v :
+    ghost_list_auth γ vs -∗
+    ghost_list_at γ i (DfracOwn 1) w ==∗
+      ghost_list_auth γ (<[i := v]> vs) ∗
+      ghost_list_at γ i (DfracOwn 1) v.
+  Proof.
+    iIntros "Hauth Hat".
+    iDestruct (ghost_list_lookup with "Hauth Hat") as %?%lookup_lt_Some.
+    iMod (ghost_map_update v with "Hauth Hat") as "(Hauth & $)".
+    rewrite insert_map_seq_0 //.
+  Qed.
+End ghost_list_G.
+
+#[global] Opaque ghost_list_auth.
+#[global] Opaque ghost_list_at.
