theories/zoo/language/tactics.v
@@ -76,6 +76,8 @@ Ltac reshape_expr e tac :=
         add_ectxi (CtxFAA1 v2) K prophs e1
     | FAA ?e1 ?e2 =>
         add_ectxi (CtxFAA2 e1) K prophs e2
+    | SetLocal ?e =>
+        add_ectxi CtxSetLocal K prophs e
     | Resolve ?e0 (Val ?v1) (Val ?v2) =>
         go K (cons (v1, v2) prophs) e0
     | Resolve ?e0 ?e1 (Val ?v2) =>
@@ -302,6 +304,11 @@ Create HintDb zoo.
 ) =>
   eapply base_step_cas_success;
   simpl
+: zoo.
+#[global] Hint Extern 0 (
+  base_step _ (Fork _) _ _ _ _ _
+) =>
+  apply base_step_fork'
 : zoo.
 #[global] Hint Extern 0 (
   base_step _ Proph _ _ _ _ _
