theories/zoo/program_logic/adequacy.v
@@ -15,16 +15,17 @@ Implicit Types e : expr.
 Implicit Types v : val.
 Implicit Types σ : state.
 
-Definition zoo_adequacy Σ `{zoo_Gpre : !ZooGpre Σ} e tid σ :
-  (if tid is Some tid then tid = 0 else True) →
+Definition zoo_adequacy `{zoo_Gpre : !ZooGpre Σ} e σ v :
+  σ.(state_locals) = [v] →
   ( ∀ `{zoo_G : !ZooG Σ},
-    ⊢ WP e ∷ tid {{ v, True }}
+    0 ↦ₗ v -∗
+    WP e ∶ 0 {{ v, True }}
   ) →
   safe ([e], σ).
 Proof.
-  intros Htid Hwp.
+  intros Hlocals Hwp.
   apply: wp_adequacy => // Hinv_G κs.
-  iMod (zoo_init' σ κs) as "(%zoo_G & Hσ)".
+  iMod (zoo_init' σ v κs) as "(%zoo_G & Hσ & Htid)"; first done.
   iExists zoo_state_interp. repeat iExists _. iFrame.
-  iApply (Hwp (Build_ZooG _)).
+  iApply (Hwp (Build_ZooG _ _) with "Htid").
 Qed.
